utils/theories/SemiLattice.v
@@ -4,37 +4,60 @@ From Stdlib Require Import Program RelationClasses Morphisms.
 From Stdlib Require Import Orders OrderedTypeAlt OrderedTypeEx MSetList MSetInterface MSetAVL MSetFacts FMapInterface MSetProperties MSetDecide.
 From MetaRocq.Utils Require Import utils NonEmptyLevelExprSet.
 
+Module CommutativeMonoid.
+  Class IsCommMonoid (A : Type) :=
+  { zero : A;
+    one : A;
+    add : A -> A -> A;
+    comm_mon :: CommutativeMonoid zero add }.
+
+  Declare Scope comm_monoid.
+  Notation "0" := zero : comm_monoid.
+  Notation "1" := one : comm_monoid.
+  Notation "+" := add : comm_monoid.
+End CommutativeMonoid.
+
 Module Semilattice.
   Declare Scope sl_scope.
   Open Scope sl_scope.
+  Delimit Scope sl_scope with sl.
+  Import CommutativeMonoid.
+  Local Open Scope comm_monoid.
 
-  Reserved Notation "x ≡ y" (at level 90).
-  Class Semilattice (carrier : Type) :=
+  Reserved Notation "x ≡ y" (at level 70).
+  Class Semilattice (carrier : Type) (incr : Type) `{CM : IsCommMonoid incr} :=
     { eq : carrier -> carrier -> Prop where "x ≡ y" := (eq x y) : sl_scope;
       eq_equiv :: Equivalence eq;
-      add : Z -> carrier -> carrier;
+      add : incr -> carrier -> carrier;
       join : carrier -> carrier -> carrier;
-      add_distr n m x : add n (add m x) ≡ add (n + m) x;
+      add_distr n m x : add n (add m x) ≡ add (CommutativeMonoid.add n m) x;
+      add_congr n x y : x ≡ y -> add n x ≡ add n y;
       add_neutral x : add 0 x ≡ x;
       join_assoc x y z : join (join x y) z ≡ join x (join y z);
       join_comm x y : join x y ≡ join y x;
       join_congr x x' y : x ≡ x' -> join x y ≡ join x' y;
       join_idem x : join x x ≡ x;
       join_sub x : join x (add 1 x) ≡ add 1 x;
-      succ_inj : forall n x y, add n x ≡ add n y -> x ≡ y;
-      succ_join : forall n x y, add n (join x y) ≡ join (add n x) (add n y);
+      add_inj : forall n x y, add n x ≡ add n y -> x ≡ y;
+      add_join : forall n x y, add n (join x y) ≡ join (add n x) (add n y);
     }.
 
-  Notation "x ≡ y" := (eq x y) (at level 90) : sl_scope.
+  Notation "x ≡ y" := (eq x y) (at level 70) : sl_scope.
 
-  Definition le {A} {SL : Semilattice A} (x y : A) := join x y ≡ y.
+  Definition le {A incr} `{SL : Semilattice A incr} (x y : A) := join x y ≡ y.
 
   Infix "≤" := le (at level 50) : sl_scope.
   Infix "∨" := join (at level 30) : sl_scope.
 
-  Local Open Scope nat_scope.
+  Definition lt {A} `{SL : Semilattice A} (x y : A) := add 1 x ≤ y.
+  Infix "<" := lt (at level 70) : sl_scope.
+
+  Class JoinDec (carrier : Type) `{SL : Semilattice carrier} :=
+    { join_dec x y : (join x y ≡ x) \/ (join y x ≡ y) }.
+
+  Local Open Scope sl_scope.
   Section Derived.
-    Context {A : Type} {SL : Semilattice A}.
+    Context {A : Type} {incr : Type} {CM : IsCommMonoid incr} {SL : Semilattice A incr}.
 
     Lemma join_congr_r x y y' : y ≡ y' -> join x y ≡ join x y'.
     Proof.
@@ -46,6 +69,9 @@ Module Semilattice.
     Proof. intros x y ? x0 y0 ?. transitivity (join y x0).
       now apply join_congr. now apply join_congr_r.
     Qed.
+
+    #[export] Instance proper_add : Proper (Logic.eq ==> eq ==> eq) add.
+    Proof. intros x y ? x0 y0 ?. subst y. now apply add_congr. Qed.
 
     Lemma le_refl x : x ≤ x.
     Proof. apply join_idem. Qed.
@@ -93,10 +119,16 @@ Module Semilattice.
       red. now rewrite -join_assoc join_idem.
     Qed.
 
+    Lemma join_le_left_trans {s t u} : s ≤ t -> s ≤ t ∨ u.
+    Proof. transitivity t => //. apply join_le_left. Qed.
+
     Lemma join_le_right {s t} : t ≤ s ∨ t.
     Proof.
       rewrite join_comm; apply join_le_left.
     Qed.
+
+    Lemma join_le_right_trans {s t u} : s ≤ u -> s ≤ t ∨ u.
+    Proof. transitivity u => //. apply join_le_right. Qed.
 
     Lemma join_le_left_eq {s t u} :
       s ∨ t ≤ u <-> s ≤ u /\ t ≤ u.
@@ -114,6 +146,26 @@ Module Semilattice.
       intros [le|le]; red in le; red.
       now rewrite -join_assoc le.
       now rewrite (join_comm t) -join_assoc le.
+    Qed.
+
+    Lemma join_dec_spec {JD : @JoinDec A incr CM SL} (x y : A) :
+      (x ≤ y /\ join x y ≡ y) \/ (y ≤ x /\ join x y ≡ x).
+    Proof.
+      destruct (join_dec x y).
+      - right. split => //.
+        red. now rewrite join_comm H.
+      - left. split => //. red.
+        rewrite join_comm H. reflexivity.
+        rewrite join_comm H. reflexivity.
+    Qed.
+
+    Lemma le_add {n} {x y : A} : x ≤ y <-> add n x ≤ add n y.
+    Proof.
+      unfold le.
+      split.
+      - now rewrite -add_join => ->.
+      - rewrite -add_join => h.
+        now apply add_inj in h.
     Qed.
 
   End Derived.
